Start fixing ProgEquiv to include Safe

src/FiatToFacade/ProgEquiv.v
@@ -1,10 +1,15 @@
+Require Import FiatToFacade.Prog FiatToFacade.Utilities.
+Require Import Facade.Facade.
 
 Definition ProgEquiv {av} p1 p2 := 
-  forall env st1 st2,
-    (@RunsTo av env p1 st1 st2 <-> RunsTo env p2 st1 st2). 
+  forall env st1,
+    (@Safe av env p1 st1 <-> Safe env p2 st1) /\ 
+    forall st2,
+      (@RunsTo av env p1 st1 st2 <-> RunsTo env p2 st1 st2). 
 
 Require Import Setoid.
-
+Require Import Program.
+  
 Add Parametric Relation {av} : (Stmt) (@ProgEquiv av)
     reflexivity proved by _
     symmetry proved by _
@@ -13,13 +18,25 @@ Add Parametric Relation {av} : (Stmt) (@ProgEquiv av)
 Proof.
   firstorder.
   firstorder.
-  unfold Transitive, ProgEquiv; intros; etransitivity; eauto.
+  unfold Transitive, ProgEquiv; split;
+  specialize (H env st1); specialize (H0 env st1); destruct_pairs.
+  rewrite H, <- H0; reflexivity.
+  intros; rewrite H2, <- H1; reflexivity.
 Qed.
 
-Show.
-
 (* Uh? *)
-unfold Transitive, ProgEquiv; intros; etransitivity; eauto.
+Proof.
+  unfold Transitive, ProgEquiv; split;
+  specialize (H env st1); specialize (H0 env st1); destruct_pairs.
+  rewrite H, <- H0; reflexivity.
+  intros; rewrite H2, <- H1; reflexivity.
+Qed.
+Proof.
+  firstorder.
+Qed.
+Proof.
+  firstorder.
+Qed.
 
 Add Parametric Morphism {av: Type} :
   (@RunsTo av)
@@ -29,6 +46,16 @@ Proof.
   unfold ProgEquiv; intros * prog_equiv ** ; apply prog_equiv; assumption.
 Qed.
 
+Add Parametric Morphism {av: Type} :
+  (@Safe av)
+    with signature (eq ==> @ProgEquiv av ==> eq ==> iff)
+      as safe_morphism.
+Proof.
+  unfold ProgEquiv; intros * prog_equiv ** ; apply prog_equiv; assumption.
+Qed.
+
+Require Import Common.
+
 Add Parametric Morphism {av} :
   (Seq)
     with signature (@ProgEquiv av ==> @ProgEquiv av ==> @ProgEquiv av)
@@ -36,12 +63,28 @@ Add Parametric Morphism {av} :
 Proof.  
   unfold ProgEquiv; intros.
 
-  split; intro runs_to; inversion_clear' runs_to; econstructor; [
-    rewrite <- H | rewrite <- H0 |
-    rewrite -> H | rewrite -> H0 ];
+  split;
+  inversion_by computes_to_inv.
+
+  (* Safe *)
+  split; intros h; inversion_clear' h;
+  constructor; split; destruct_pairs;
+  try intros st' runs_to.
+  firstorder.
+  rewrite <- H3 in runs_to.
+  rewrite <- H1; intuition.
+  firstorder.
+  rewrite -> H3 in runs_to.
+  rewrite -> H1; intuition.
+
+  (* RunsTo *)
+  split; intros runs_to; inversion_clear' runs_to; econstructor;
+  [ rewrite <- H3 | rewrite <- H2 |
+    rewrite -> H3 | rewrite -> H2 ];
   eauto; reflexivity.
 Qed.
 
+(*
 Lemma while_morph {av env} :
   forall while_p1,
   forall (st1 st2: State av),
@@ -93,3 +136,4 @@ Proof.
   inversion_clear' H; inversion_clear' H5; eauto.
   repeat (econstructor; eauto).
 Qed.
+*)
